complete CBOR.Spec.Type

src/cbor/CBOR.Spec.Type.fst
@@ -12,6 +12,7 @@ let cbor_prop (x: R.raw_data_item) : Tot prop =
 
 let cbor = (x: R.raw_data_item { cbor_prop x })
 
+unfold
 let cbor_map_prop (x: list (R.raw_data_item & R.raw_data_item)) : Tot prop =
   List.Tot.for_all (U.holds_on_pair R.raw_data_item_ints_optimal) x == true /\
   List.Tot.for_all (U.holds_on_pair (R.raw_data_item_sorted R.deterministically_encoded_cbor_map_key_order)) x == true /\
@@ -88,6 +89,14 @@ let rec cbor_map_length m =
       else ()
     in
     1 + cbor_map_length q
+
+let rec cbor_map_length_eq
+  (m: cbor_map)
+: Lemma
+  (cbor_map_length m == List.Tot.length m)
+= match m with
+  | [] -> ()
+  | _ :: q -> cbor_map_length_eq q
 
 let cbor_map_empty = []
 
@@ -168,11 +177,142 @@ let rec cbor_map_get_filter'
         match cbor_map_get (cbor_map_filter f q) k with
         | None -> ()
         | Some v' ->
-          admit ();
-          List.Tot.assoc_memP_some a v' q;
+          List.Tot.assoc_memP_some a v' (cbor_map_filter f q);
           CBOR.Spec.Util.list_sorted_memP (R.map_entry_order R.deterministically_encoded_cbor_map_key_order _) (a, v) q (a, v')
       end
     end
     else cbor_map_get_filter' f q k
 
 let cbor_map_get_filter = cbor_map_get_filter'
+
+let cbor_map_diff_f (m1: cbor_map) (k v: cbor) : Tot bool =
+  None? (cbor_map_get m1 k)
+
+let cbor_map_union m1 m2 =
+  let m2' = cbor_map_filter (cbor_map_diff_f m1) m2 in
+  List.Tot.for_all_mem (U.holds_on_pair R.raw_data_item_ints_optimal) m1;
+  List.Tot.for_all_mem (U.holds_on_pair R.raw_data_item_ints_optimal) m2';
+  List.Tot.for_all_mem (U.holds_on_pair (R.raw_data_item_sorted R.deterministically_encoded_cbor_map_key_order)) m1;
+  List.Tot.for_all_mem (U.holds_on_pair (R.raw_data_item_sorted R.deterministically_encoded_cbor_map_key_order)) m2';
+  Classical.forall_intro (List.Tot.append_memP m1 m2');
+  let m' = m1 `List.Tot.append` m2' in
+  CBOR.Spec.Raw.Map.list_sorted_map_entry_order_no_repeats R.deterministically_encoded_cbor_map_key_order m1;
+  CBOR.Spec.Raw.Map.list_sorted_map_entry_order_no_repeats R.deterministically_encoded_cbor_map_key_order m2';
+  assert (List.Tot.no_repeats_p (List.Tot.map fst m1));
+  assert (List.Tot.no_repeats_p (List.Tot.map fst m2'));
+  let prf
+    (x: R.raw_data_item)
+  : Lemma
+    (requires (List.Tot.memP x (List.Tot.map fst m1)))
+    (ensures (~ (List.Tot.memP x (List.Tot.map fst m2'))))
+  = List.Tot.assoc_mem x m1;
+    List.Tot.assoc_mem x m2';
+    if Some? (List.Tot.assoc x m2')
+    then begin
+      list_assoc_cbor x m2';
+      cbor_map_get_filter (cbor_map_diff_f m1) m2' x
+    end
+  in
+  Classical.forall_intro (Classical.move_requires prf);
+  List.Tot.no_repeats_p_append (List.Tot.map fst m1) (List.Tot.map fst m2');
+  List.Tot.map_append fst m1 m2';
+  let res = R.cbor_map_sort_failsafe m' in
+  List.Tot.for_all_mem (U.holds_on_pair R.raw_data_item_ints_optimal) res;
+  List.Tot.for_all_mem (U.holds_on_pair (R.raw_data_item_sorted R.deterministically_encoded_cbor_map_key_order)) res;
+  res
+
+let cbor_map_get_union m1 m2 k =
+  let m2' = cbor_map_filter (cbor_map_diff_f m1) m2 in
+  R.cbor_map_sort_failsafe_correct (List.Tot.append m1 m2');
+  CBOR.Spec.Raw.Map.list_sorted_map_entry_order_no_repeats R.deterministically_encoded_cbor_map_key_order (cbor_map_union m1 m2);
+  CBOR.Spec.Util.list_assoc_append k m1 m2';
+  cbor_map_get_filter (cbor_map_diff_f m1) m2 k
+
+let rec list_cbor_of_cbor_list
+  (l: list R.raw_data_item {
+    List.Tot.for_all (R.holds_on_raw_data_item R.raw_data_item_ints_optimal_elem) l == true /\
+    List.Tot.for_all (R.holds_on_raw_data_item (R.raw_data_item_sorted_elem R.deterministically_encoded_cbor_map_key_order)) l == true
+  })
+: Pure (list cbor)
+    (requires True)
+    (ensures (fun l' -> List.Tot.length l' == List.Tot.length l))
+= match l with
+  | [] -> []
+  | a :: q -> a :: list_cbor_of_cbor_list q
+
+let unpack m =
+  assert_norm (R.raw_data_item_ints_optimal == R.holds_on_raw_data_item R.raw_data_item_ints_optimal_elem);
+  assert_norm (R.raw_data_item_sorted R.deterministically_encoded_cbor_map_key_order == R.holds_on_raw_data_item (R.raw_data_item_sorted_elem R.deterministically_encoded_cbor_map_key_order));
+  R.holds_on_raw_data_item_eq R.raw_data_item_ints_optimal_elem m;
+  R.holds_on_raw_data_item_eq (R.raw_data_item_sorted_elem R.deterministically_encoded_cbor_map_key_order) m;
+  match m with
+  | R.Simple v -> CSimple v
+  | R.Int64 ty v -> CInt64 ty v.value
+  | R.String ty len v -> CString ty v
+  | R.Array len v -> CArray (list_cbor_of_cbor_list v)
+  | R.Map len v ->
+    cbor_map_length_eq v;
+    CMap v
+  | R.Tagged tag v -> CTagged tag.value v
+
+let rec cbor_list_of_list_cbor
+  (l: list cbor)
+: Pure (list R.raw_data_item)
+    (requires True)
+    (ensures (fun l' -> List.Tot.length l' == List.Tot.length l /\
+      List.Tot.for_all (R.holds_on_raw_data_item R.raw_data_item_ints_optimal_elem) l' == true /\
+      List.Tot.for_all (R.holds_on_raw_data_item (R.raw_data_item_sorted_elem R.deterministically_encoded_cbor_map_key_order)) l' == true    
+    ))
+= match l with
+  | [] -> []
+  | a :: q -> a :: cbor_list_of_list_cbor q
+
+let pack x =
+  let m : R.raw_data_item = match x with
+  | CSimple v -> R.Simple v
+  | CInt64 ty v -> R.Int64 ty (R.mk_raw_uint64 v)
+  | CString ty v -> R.String ty (R.mk_raw_uint64 (U64.uint_to_t (Seq.length v))) v
+  | CArray v -> R.Array (R.mk_raw_uint64 (U64.uint_to_t (List.Tot.length v))) (cbor_list_of_list_cbor v)
+  | CMap v ->
+    cbor_map_length_eq v;
+    R.Map (R.mk_raw_uint64 (U64.uint_to_t (List.Tot.length v))) v
+  | CTagged tag v -> R.Tagged (R.mk_raw_uint64 tag) v
+  in
+  assert_norm (R.raw_data_item_ints_optimal == R.holds_on_raw_data_item R.raw_data_item_ints_optimal_elem);
+  assert_norm (R.raw_data_item_sorted R.deterministically_encoded_cbor_map_key_order == R.holds_on_raw_data_item (R.raw_data_item_sorted_elem R.deterministically_encoded_cbor_map_key_order));
+  R.holds_on_raw_data_item_eq R.raw_data_item_ints_optimal_elem m;
+  R.holds_on_raw_data_item_eq (R.raw_data_item_sorted_elem R.deterministically_encoded_cbor_map_key_order) m;
+  m
+
+let rec cbor_list_of_list_cbor_of_cbor_list
+  (l: list R.raw_data_item {
+    List.Tot.for_all (R.holds_on_raw_data_item R.raw_data_item_ints_optimal_elem) l == true /\
+    List.Tot.for_all (R.holds_on_raw_data_item (R.raw_data_item_sorted_elem R.deterministically_encoded_cbor_map_key_order)) l == true
+  })
+: Lemma
+  (cbor_list_of_list_cbor (list_cbor_of_cbor_list l) == l)
+= match l with
+  | [] -> ()
+  | _ :: q -> cbor_list_of_list_cbor_of_cbor_list q
+
+let rec list_cbor_of_cbor_list_of_list_cbor
+  (l: list cbor)
+: Lemma
+  (list_cbor_of_cbor_list (cbor_list_of_list_cbor l) == l)
+= match l with
+  | [] -> ()
+  | _ :: q -> list_cbor_of_cbor_list_of_list_cbor q
+
+let unpack_pack c = match c with
+  | CArray v -> list_cbor_of_cbor_list_of_list_cbor v
+  | _ -> ()
+
+let pack_unpack c = match c with
+  | R.Simple _ -> ()
+  | R.Int64 _ v
+  | R.Tagged v _
+  | R.Map v _
+  | R.String _ v _ -> R.raw_uint64_optimal_unique v (R.mk_raw_uint64 v.value)
+  | R.Array len v ->
+    R.raw_uint64_optimal_unique len (R.mk_raw_uint64 len.value);
+    cbor_list_of_list_cbor_of_cbor_list v
